Loom/PredTrans.lean
@@ -3,7 +3,7 @@ import Loom.Post
 
 open Lean.Order
 
-universe u v w x
+-- universe u v w x
 
 /-!
 # Exception Continuation Monad
@@ -62,6 +62,10 @@ def PredTrans.pushExcept {α : Type u} {ε : Type v} {l : Type w} {e : Type z}
     (x : PredTrans l e (Except ε α)) : PredTrans l (EPost.cons (ε → l) e) α :=
   fun post epost => x (epost.pushExcept post) epost.tail
 
+instance {ε : Type v} {l : Type w} {e : Type z} :
+  MonadLift (PredTrans l e) (PredTrans l (EPost.cons (ε → l) e)) where
+  monadLift x := PredTrans.pushExcept fun post epost => x (post <| .ok ·) epost
+
 /--
 Adds the ability to make assertions about a state of type `σ` to a predicate transformer with
 postcondition shape `es`, resulting in a transformer over `σ → l`.
@@ -70,7 +74,47 @@ def pushArg {σ : Type u} {l : Type v} {e : Type w} {α : Type z}
     (x : σ → PredTrans l e (α × σ)) : PredTrans (σ → l) e α :=
   fun post epost s => x s (fun (a, s) => post a s) epost
 
+instance {σ : Type u} {l : Type v} {e : Type w}
+  : MonadLift (PredTrans l e) (PredTrans (σ → l) e) where
+  monadLift x := pushArg fun s post epost => x (fun x => post (x, s)) epost
+
 @[simp, grind =]
 theorem apply_pushArg {σ : Type u} {l : Type v} {e : Type w} {α : Type z}
     (x : σ → PredTrans l e (α × σ)) (post : α → σ → l) (epost : e) (s : σ) :
   (pushArg x) post epost s = x s (fun (a, s) => post a s) epost := rfl
+
+instance {σ : Type u} {l : Type v} {e : Type w} : MonadLift (PredTrans l e) (PredTrans (σ → l) e) where
+  monadLift x := fun post epost s => x (fun a => post a s) epost
+
+instance (priority := high) {ε : Type u} {l : Type u} {e : Type u} : MonadLift.{u, u, u} (PredTrans l e) (PredTrans l (EPost.cons.{u, u} (ε → l) e)) where
+  monadLift x := fun post epost => x post epost.tail
+
+
+instance {σ : Type u} {l : Type v} {e : Type w} : MonadStateOf σ (PredTrans (σ → l) e) where
+  get := fun post _epost => fun s => post s s
+  set s := fun post _epost => fun _ => post ⟨⟩ s
+  modifyGet f := fun post _epost => fun s => post (f s).1 (f s).2
+
+instance {σ : Type u} {l : Type v} {e : Type w} : MonadReaderOf σ (PredTrans (σ → l) e) where
+  read := fun post _epost => fun s => post s s
+
+instance {ε : Type u} {l : Type v} {e : Type w} : MonadExceptOf ε (PredTrans l (EPost.cons (ε → l) e)) where
+  throw e := fun _post epost => epost.head e
+  tryCatch x handle := fun post epost => x post ⟨(handle · post epost), epost.tail⟩
+
+instance {ε : Type u} {l : Type v} {e : Type w} {σ : Type z}
+  [MonadExceptOf ε (PredTrans l e)] : MonadExceptOf ε (PredTrans (σ → l) e) where
+  throw e := pushArg fun _ => throw e
+  tryCatch x handle := pushArg fun s =>
+    tryCatch
+      (fun post epost => x (fun r s => post (r, s)) epost s)
+      (fun e post epost => handle e (fun r s => post (r, s)) epost s)
+
+instance {ε : Type u} {l : Type v} {e : Type w} {ε' : Type u}
+  [MonadExceptOf ε (PredTrans l e)] :
+  MonadExceptOf ε (PredTrans l (EPost.cons (ε' → l) e)) where
+  throw e := PredTrans.pushExcept <| throw e
+  tryCatch x handle := PredTrans.pushExcept <|
+    tryCatch
+      (fun post epost => x (fun a => post (.ok a)) ⟨fun e => post (.error e), epost⟩)
+      (fun e post epost => handle e (fun r => post (.ok r)) ⟨fun e => post (.error e), epost⟩)
